NuSys.thy
@@ -39,6 +39,7 @@ consts key_of :: " 'a \<Rightarrow> 'b "
 
 datatype ('a, 'b) object (infixr "\<R_arr_tail>" 60) = object (key_of_obj: 'a) (val_of_obj: 'b) (infixr "\<R_arr_tail>" 60)
 adhoc_overloading key_of key_of_obj and val_of val_of_obj
+declare object.sel[iff]
 
 lemma object_forall[lrep_exps]: "All P \<longleftrightarrow> (\<forall>a x. P (a \<R_arr_tail> x))" by (metis object.exhaust)
 lemma object_exists[lrep_exps]: "Ex P \<longleftrightarrow> (\<exists>a x. P (a \<R_arr_tail> x))" by (metis object.exhaust)
